Examples/Calculator/CalculatorClientLib.v
@@ -43,7 +43,7 @@ Variable cl : nid.
 Hypothesis  Hc : cl \in cls.
 
 Program Definition tryrecv_resp_act := act (@tryrecv_action_wrapper W cl
-      (fun k t b => (k == l) && (t == resp)) _).
+      (fun k _ t b => (k == l) && (t == resp)) _).
 Next Obligation. by case/andP:H=>/eqP->; rewrite gen_domPt inE/=. Qed.
 
 Notation loc i := (getLocal cl (getStatelet i l)).
